specs/Spec.HSalsa20.fst
@@ -1,0 +1,48 @@
+module Spec.HSalsa20
+
+open FStar.Mul
+open FStar.Seq
+open FStar.UInt32
+open FStar.Endianness
+open Spec.Lib
+
+let keylen = 32 (* in bytes *)
+let blocklen = 64  (* in bytes *)
+let noncelen = 16  (* in bytes *)
+
+type key = lbytes keylen
+type nonce = lbytes noncelen
+type block = lbytes blocklen
+
+type state = Spec.Salsa20.state
+
+#set-options "--initial_fuel 0 --max_fuel 0 --z3rlimit 100"
+
+let setup (k:key) (n:nonce): state =
+  let ks = uint32s_from_le 8 k in
+  let ns = uint32s_from_le 4 n in
+  let st = create 16 0ul in
+  let st = upd st 0  Spec.Salsa20.constant0 in
+  let st = upd st 5  Spec.Salsa20.constant1 in 
+  let st = upd st 10 Spec.Salsa20.constant2 in 
+  let st = upd st 15 Spec.Salsa20.constant3 in 
+  let st = upd st 1  (index ks 0) in
+  let st = upd st 2  (index ks 1) in 
+  let st = upd st 3  (index ks 2) in 
+  let st = upd st 4  (index ks 3) in 
+  let st = upd st 11  (index ks 4) in
+  let st = upd st 12  (index ks 5) in 
+  let st = upd st 13  (index ks 6) in 
+  let st = upd st 14  (index ks 7) in 
+  let st = upd st 6  (index ns 0) in 
+  let st = upd st 7  (index ns 1) in 
+  let st = upd st 8  (index ns 2) in 
+  let st = upd st 9  (index ns 3) in 
+  st
+
+let hsalsa20 (k:key) (n:nonce) : key = 
+  let st = setup k n in
+  let st' = Spec.Salsa20.rounds st in
+  let hs = createL [index st' 0; index st' 5; index st' 10; index st' 15; 
+      	   	    index st' 6; index st' 7; index st' 8; index st' 9] in
+  uint32s_to_le 8 hs
