specs/Spec.SecretBox.fst
@@ -1,0 +1,53 @@
+module Spec.SecretBox
+
+open FStar.Seq
+open FStar.UInt32
+open FStar.Endianness
+open Spec.Lib
+
+let keylen =   32 (* in bytes *)
+let noncelen = 24 (* in bytes *)
+
+type key = lbytes keylen
+type nonce = lbytes noncelen
+type bytes = seq UInt8.t
+
+#set-options "--initial_fuel 0 --max_fuel 0 --z3rlimit 30"
+val secretbox_detached: m:bytes{length m / Spec.Salsa20.blocklen < pow2 32} ->
+    k:key -> n:nonce -> Tot (lbytes (length m) * Spec.Poly1305.tag) 
+let secretbox_detached m k n = 
+    let (n1,n2) = split n 16 in
+    let subkey:Spec.Salsa20.key = Spec.HSalsa20.hsalsa20 k n1 in
+    let b0 = Spec.Salsa20.salsa20_block k n2 0 in
+    let mackey = slice b0 0 32 in
+    let mlen = length m in
+    let mlen0 = if mlen < 32 then mlen else 32 in
+    let (m0,rest) = split m mlen0 in
+    let b0 = create 32 0uy @| m0 in
+    let c0 = Spec.Salsa20.salsa20_encrypt_bytes subkey n2 0 b0 in
+    let c0 = slice c0 32 64 in
+    let crest = Spec.Salsa20.salsa20_encrypt_bytes subkey n2 1 rest in
+    let cipher = c0 @| crest in
+    let mac = Spec.Poly1305.poly1305 cipher mackey in
+    (cipher, mac)
+            
+val secretbox_open_detached: c:bytes{length c / Spec.Salsa20.blocklen < pow2 32} ->
+    mac:Spec.Poly1305.tag -> k:key -> n:nonce -> Tot (option (lbytes (length c)))
+let secretbox_open_detached cipher mac k n = 
+    let (n1,n2) = split n 16 in
+    let subkey = Spec.HSalsa20.hsalsa20 k n1 in
+    let b0 = Spec.Salsa20.salsa20_block k n2 0 in
+    let mackey = slice b0 0 32 in
+    let xmac = Spec.Poly1305.poly1305 cipher mackey in
+    if xmac = mac then 
+      let clen = length cipher in
+      let clen0 = if clen < 32 then clen else 32 in
+      let c0,crest = split cipher clen0 in
+      let b0 = create 32 0uy @| c0 in
+      let m0 = Spec.Salsa20.salsa20_encrypt_bytes subkey n2 0 b0 in
+      let m0 = slice m0 32 (32+clen0) in
+      let mrest = Spec.Salsa20.salsa20_encrypt_bytes subkey n2 1 crest in
+      Some (m0 @| mrest)
+    else None
+
+let test() = true
